fix equivalence

theories/Properties/Equivalence.v
@@ -2,16 +2,18 @@ From Corelib.Properties Require Import GroupoidLaws.
 
 Notation "f ∘ g" := (fun x => f (g x)) (at level 55).
 
+Notation "f == g" := (forall x, f x = g x) (at level 55).
+
 Section Equivalence.
-  Sorts sa sb se.
+  Sorts sa sb.
   Universes a b.
   Context (A : Type@{sa|a}) (B: Type@{sb|b}).
 
   Record isEquiv (f : A -> B) := {
       sect : B -> A ;
       retr : B -> A ;
-      sect_eq : forall b, eq@{_ se| _} (f (sect b)) b ;
-      retr_eq : forall a, eq@{_ se| _} (retr (f a)) a ;
+      sect_eq : f ∘ sect == id ;
+      retr_eq : retr ∘ f == id ;
     }.
 
   Record equiv := { map :> A -> B ; map_is_equiv :> isEquiv map }.
@@ -25,63 +27,12 @@ Arguments retr_eq {_ _ _} _.
 
 Import GroupoidNotations.
 Definition equiv_refl@{sa|a|} (A : Type@{sa|a}) : equiv A A :=
-  {| map := id ; map_is_equiv := {| sect := id ; retr := id ; sect_eq := fun _ => eq_refl ; retr_eq := fun _ => rfl |} |}.
-
+  {| map := id ; map_is_equiv := {| sect := id ; retr := id ; sect_eq := rfl ; retr_eq := rfl |} |}.
 
 Definition equiv_trans@{sa sb sc|a b c|} (A : Type@{sa|a}) (B : Type@{sb|b}) (C : Type@{sc|c}) (AB : equiv A B) (BC : equiv B C) : equiv A C.
 Proof.
-  refine {| map := BC ∘ AB |}.
-  simple refine {| sect := AB.(sect) ∘ BC.(sect) ; retr := AB.(retr) ∘ BC.(retr) |}.
-  all: intros; cbn.
-  - rewrite sect_eq; apply sect_eq.
-  - rewrite retr_eq; apply retr_eq.
+  unshelve refine (Build_equiv _ _ (BC ∘ AB) _).
+  unshelve refine (Build_isEquiv A C _ (AB.(sect) ∘ BC.(sect)) (AB.(retr) ∘ BC.(retr)) _ _).
+  - intro. rewrite sect_eq. refine (sect_eq _ _).
+  - intro. rewrite retr_eq. refine (retr_eq _ _).
 Defined.
-
-
-Set Printing Universes.
-
-Section SigmaAssoc.
-  Sorts a b c.
-  Universes a b c.
-  Context (A : Type@{a|a}) (B : A -> Type@{b|b}) (C : forall a, B a -> Type@{c|c}).
-
-  (* All Sigma types in Type *)
-  Let T1 := Σ (a : A) (b : B a), C a b.
-  Let T2 := Σ (p : Σ (a : A), B a), C (π1 p) (π2 p).
-
-  Let f12 (t : T1) : T2 := let '(a, b, c) := t in ((a, b), c).
-  Let f21 (t : T2) : T1 := let '((a,b), c) := t in (a, b, c).
-
-  Let f12_is_equiv : isEquiv _ _ f12.
-  Proof.
-    refine {| sect := f21 ; retr := f21 |}.
-    - intros [[a b] c]; reflexivity.
-    - intros (a & b & c); reflexivity.
-  Defined.
-
-  Definition sigma_type_assoc : equiv T1 T2 :=
-    {| map := f12 ; map_is_equiv := f12_is_equiv |}.
-End SigmaAssoc.
-
-Section SigmaAssocHom.
-  Sorts s.
-  Universes a b c.
-  Context (A : Type@{s|a}) (B : A -> Type@{s|b}) (C : forall a, B a -> Type@{s|c}).
-
-  (* All Sigma types in sort s *)
-  Let T1 := sigma@{s s s|_ _} A (fun a => sigma@{s s s|_ _} (B a) (C a)).
-  Let T2 := sigma@{s s s|_ _} (sigma@{s s s|_ _} A B) (fun p => C (projT1 p) (projT2 p)).
-
-  Definition f12 (t : T1) : T2 := let '(a, b, c) := t in ((a, b), c).
-  Definition f21 (t : T2) : T1 := let '((a,b), c) := t in (a, b, c).
-
-  Definition f12_is_equiv : isEquiv@{s s s| _ _} _ _ f12.
-  Proof.
-    refine {| sect := f21 ; retr := f21 |}.
-    - intros [[a b] c]; reflexivity.
-    - intros (a & b & c); reflexivity.
-  Defined.
-
-  Definition sigma_hom_assoc : equiv T1 T2 :=
-    {| map := f12 ; map_is_equiv := f12_is_equiv |}.
-End SigmaAssocHom.
